refinedVST/lithium/all.v
@@ -1,5 +1,5 @@
 From lithium Require Export normalize.
-From VST.lithium Require Export definitions simpl_classes simpl_instances proof_state interpreter (* solvers *) syntax (* instances *) (* lvar *).
+From VST.lithium Require Export definitions simpl_classes simpl_instances proof_state interpreter solvers syntax instances lvar.
 
 (** This file reexports all files from Lithium except [hooks.v] such
 that the definitions from [hooks.v] don't accidentally override the redefinitions. *)
