refinedVST/lithium/instances.v
@@ -1,0 +1,172 @@
+From lithium Require Export base.
+From VST.lithium Require Import syntax definitions proof_state.
+
+(** This file collects the default instances for the definitions in
+[definitions.v]. Note that these instances must be in a separate file
+since the instances are defined using the notation from
+[proof_state.v]. *)
+
+(** * [find_in_context] *)
+Lemma find_in_context_direct {prop:bi} {B} P (T : B → prop):
+  find_in_context (FindDirect P) T :- pattern: x, P x; return T x.
+Proof. done. Qed.
+Definition find_in_context_direct_inst := [instance @find_in_context_direct with FICSyntactic].
+Global Existing Instance find_in_context_direct_inst | 1.
+
+(** * Simplification *)
+Lemma simplify_hyp_id {prop:bi} (P : prop)  `{Affine prop P} (T : prop):
+  simplify_hyp P T :- return T.
+Proof. iIntros "HT Hl". iFrame. Qed.
+Definition simplify_hyp_id_inst (prop:bi) (P : prop) `{affine_p: Affine prop P}:=
+  [instance simplify_hyp_id P as SimplifyHyp P None].
+Global Existing Instance simplify_hyp_id_inst | 100.
+
+Lemma simplify_goal_id {prop:bi} (P : prop) T :
+  simplify_goal P T :- exhale P; return T.
+Proof. iIntros "$". Qed.
+Definition simplify_goal_id_inst (prop:bi) (P : prop) :=
+  [instance simplify_goal_id P as SimplifyGoal P None].
+Global Existing Instance simplify_goal_id_inst | 100.
+
+(** * Subsumption *)
+Lemma subsume_id {prop:bi} {A} (P : prop) (T : A → prop):
+  subsume P (λ _, P) T :- ∃ x, return T x.
+Proof. iIntros "[% ?] $". by iExists _. Qed.
+Definition subsume_id_inst := [instance @subsume_id].
+Global Existing Instance subsume_id_inst | 1.
+
+Lemma subsume_simplify {prop:bi} {A} (P1 : prop) (P2 : A → prop) o1 o2 T :
+  (* TCOneIsSome must be first here since [instance ...] reverse the order *)
+  ∀ `{!TCOneIsSome o1 o2} {SH : SimplifyHyp P1 o1} {SG : ∀ x, SimplifyGoal (P2 x) o2},
+    let GH := (SH (∃ x, P2 x ∗ T x)%I).(i2p_P) in
+    let GG := (P1 -∗ ∃ x, (SG x (T x)).(i2p_P))%I in
+    let G :=
+       match o1, o2 with
+     | Some n1, Some n2 => if (n2 ?= n1)%N is Lt then GG else GH
+     | Some n1, _ => GH
+     | _, _ => GG
+       end in
+    subsume P1 P2 T :- return G.
+Proof.
+  iIntros (???) "/= Hs Hl".
+  destruct o1 as [n1|], o2 as [n2|] => //. 1: case_match.
+  1,3,4: by iDestruct (i2p_proof with "Hs Hl") as "Hsub".
+  all: iDestruct ("Hs" with "Hl") as (?) "HSG"; iExists _.
+  all: iDestruct (i2p_proof with "HSG") as "$".
+Qed.
+Definition subsume_simplify_inst := [instance @subsume_simplify].
+Global Existing Instance subsume_simplify_inst | 1000.
+
+(** * sep_list *)
+
+Global Instance sep_list_related_to (prop:bi) A B id ig l f :
+  @RelatedTo prop _ (λ x : B, sep_list id A (ig x) (l x) (f x)) :=
+  {| rt_fic := FindSepList id |}.
+
+Lemma find_sep_list {prop:bi} id (T : _ → prop):
+  find_in_context (FindSepList id) T :-
+    pattern: A ig l f, sep_list id A ig l f; return T (sep_list id A ig l f).
+Proof. iIntros "(%&%&%&%&?&?)". iExists _. by iFrame. Qed.
+Definition find_sep_list_inst := [instance @find_sep_list with FICSyntactic].
+Global Existing Instance find_sep_list_inst | 1.
+
+Lemma subsume_sep_list_eq {prop:bi} {_:BiPositive prop} {B} A id ig (l1 : list A) (l2 : B → list A) f (T : B → prop) :
+  subsume (sep_list id A ig l1 f) (λ x : B, sep_list id A ig (l2 x) f) T :-
+    ∃ x, exhale <affine> ⌜list_subequiv ig l1 (l2 x)⌝; return T x.
+Proof.
+  unfold sep_list. iDestruct 1 as (b Hequiv) "HT".  iIntros "[%Hln Hl]". iExists b. iFrame "HT".
+  set (l2' := (l2 b)) in *. clearbody l2'; clear l2; rename l2' into l2.
+  have [Hlen _]:= Hequiv 0. iSplit; first by iPureIntro; congruence. clear Hln.
+  iInduction l1 as [|x l1] "IH" forall (f ig l2 Hlen Hequiv); destruct l2 => //=.
+  (* rewrite bi.affinely_sep. *)
+  iDestruct "Hl" as "[Hx Hl]". move: Hlen => /= [?].
+  iSplitL "Hx".
+  - case_bool_decide as Hb => //. have [_ /= Heq]:= Hequiv 0. by  move: (Heq Hb) => [->].
+  - iDestruct ("IH" $! (f ∘ S) (pred <$> (filter (λ x, x ≠ 0%nat) ig)) l2 with "[//] [%] [Hl]") as "Hl". {
+      move => i. split => // Hin. move: (Hequiv (S i)) => [_ /= {}Hequiv]. apply: Hequiv.
+      contradict Hin. apply elem_of_list_fmap. eexists (S i). split => //.
+        by apply elem_of_list_filter.
+    }
+    + iApply (big_sepL_impl with "Hl"). iIntros "!>" (k ??) "Hl".
+      case_bool_decide as Hb1; case_bool_decide as Hb2 => //.
+      contradict Hb2. apply elem_of_list_fmap. eexists (S k). split => //.
+      by apply elem_of_list_filter.
+    + iApply (big_sepL_impl with "Hl"). iIntros "!>" (k ??) "Hl".
+      case_bool_decide as Hb1; case_bool_decide as Hb2 => //.
+      contradict Hb2. move: Hb1 => /elem_of_list_fmap[[|?][? /elem_of_list_filter [??]]] //.
+      by simplify_eq/=.
+Qed.
+Definition subsume_sep_list_eq_inst := [instance @subsume_sep_list_eq].
+Global Existing Instance subsume_sep_list_eq_inst | 1000.
+
+Lemma subsume_sep_list_insert_in_ig {prop:bi} {B} A id ig i x (l1 : list A) (l2 : B → list A)
+  (f : nat → A → prop) (T : B → prop) :
+  subsume (sep_list id A ig (<[i := x]>l1) f) (λ x : B, sep_list id A ig (l2 x) f) T
+     where `{!CanSolve (i ∈ ig)} :-
+  return subsume (sep_list id A ig l1 f) (λ x : B, sep_list id A ig (l2 x) f) T.
+Proof.
+  unfold CanSolve, sep_list => ?. iIntros "Hsub [<- Hl]".
+  rewrite insert_length. iApply "Hsub". iSplit; [done|].
+  destruct (decide (i < length l1)%nat). 2: { by rewrite list_insert_ge; [|lia]. }
+  iDestruct (big_sepL_insert_acc with "Hl") as "[? Hl]". { by apply: list_lookup_insert. }
+  have [//|y ?]:= lookup_lt_is_Some_2 l1 i.
+  iDestruct ("Hl" $! y with "[]") as "Hl". { by case_decide. }
+  destruct (bool_decide (i∈ig)); by rewrite list_insert_insert list_insert_id.
+Qed.
+Definition subsume_sep_list_insert_in_ig_inst := [instance @subsume_sep_list_insert_in_ig].
+Global Existing Instance subsume_sep_list_insert_in_ig_inst.
+
+Lemma subsume_sep_list_insert_not_in_ig {prop:bi} A B id ig i x (l1 : list A) l2 (f : nat → A → prop) (T : B → prop) :
+  subsume (sep_list id A ig (<[i := x]>l1) f) (λ x : B, sep_list id A ig (l2 x) f) T
+    where `{!CanSolve (i ∉ ig)} :-
+      exhale <affine> ⌜i < length l1⌝%nat;
+      inhale <affine> f i x;
+      y ← (sep_list id A (i :: ig) l1 f) :>> (λ x : B, sep_list id A (i :: ig) (l2 x) f);
+      ∃ x2, exhale <affine> ⌜l2 y !! i = Some x2⌝;
+      exhale <affine> f i x2;
+      return T y.
+Proof.
+  unfold CanSolve, sep_list. iIntros (?) "[% Hsub] [<- Hl]". rewrite big_sepL_insert // insert_length.
+  iDestruct "Hl" as "[Hx Hl]". case_bool_decide => //.
+  iDestruct ("Hsub" with "Hx [Hl]") as "[% [[%Heq Hl] [% [% [? HT]]]]]". {
+    iSplit; [done|]. iApply (big_sepL_impl with "Hl"). iIntros "!>" (???) "?".
+    repeat case_decide => //; set_solver.
+  }
+  iExists _. iFrame. iSplit; [done|].
+  rewrite -{2}(list_insert_id (l2 _) i x2) // big_sepL_insert; [|lia]. case_bool_decide => //. iFrame.
+  iApply (big_sepL_impl with "Hl"). iIntros "!>" (???) "?".
+  repeat case_decide => //; set_solver.
+Qed.
+Definition subsume_sep_list_insert_not_in_ig_inst := [instance @subsume_sep_list_insert_not_in_ig].
+Global Existing Instance subsume_sep_list_insert_not_in_ig_inst.
+
+Lemma subsume_sep_list_trivial_eq {prop:bi} A B id ig (l : list A) (f : nat → A → prop) (T : B → prop) :
+  subsume (sep_list id A ig l f) (λ x : B, sep_list id A ig l f) T :- ∃ x, return T x.
+Proof. iIntros "[% ?] $". iExists _. by iFrame. Qed.
+Definition subsume_sep_list_trivial_eq_inst := [instance @subsume_sep_list_trivial_eq].
+Global Existing Instance subsume_sep_list_trivial_eq_inst | 5.
+
+Lemma subsume_sep_list_cons {prop:bi} A B id ig (x1 : A) (l1 : list A) l2 (f : nat → A → prop) (T : B → prop) :
+  subsume (sep_list id A ig (x1 :: l1) f) (λ y : B, sep_list id A ig (l2 y) f) T :-
+    exhale <affine> ⌜0 ∉ ig⌝;
+    ∀ id', inhale (<affine> f 0%nat x1);
+    inhale (sep_list id' A (pred <$> ig) l1 (λ i, f (S i)));
+    ∃ y x2 l2', exhale <affine> ⌜l2 y = x2 :: l2'⌝;
+    exhale (<affine> f 0%nat x2);
+    exhale (sep_list id' A (pred <$> ig) l2' (λ i, f (S i)));
+    return T y.
+Proof.
+  unfold sep_list. iIntros "[% Hs] [<- Hl]".
+  rewrite !big_sepL_cons /=. case_bool_decide => //. iDestruct "Hl" as "[H0 H]".
+  iDestruct ("Hs" $! {|sep_list_len := _|} with "H0 [H]") as (??? Heq1) "[? [[%Heq2 H] ?]]".
+  { iSplit; [simpl; done|]. iApply (big_sepL_impl with "H"); iIntros "!#" (???) "?".
+    case_bool_decide as Hx1 => //; case_bool_decide as Hx2 => //; contradict Hx2.
+    set_unfold. eexists _. split; [|done]. done. }
+  iExists _. iFrame. iSplit. { iPureIntro. rewrite Heq1 /=. by rewrite Heq2. }
+  rewrite Heq1 => /=. rewrite bool_decide_false //. iFrame.
+  iApply (big_sepL_impl with "H"); iIntros "!#" (???) "?".
+  case_bool_decide as Hx1 => //; case_bool_decide as Hx2 => //; contradict Hx2.
+  by move: Hx1 => /(elem_of_list_fmap_2 _ _ _)[[|?]//=[->?]].
+Qed.
+Definition subsume_sep_list_cons_inst := [instance @subsume_sep_list_cons].
+Global Existing Instance subsume_sep_list_cons_inst | 40.
